Update the hashmap_on_disk example

tests/hashmap_on_disk/HashmapMain.Clauses.Template.fst
@@ -9,55 +9,55 @@ open HashmapMain.Types
 (** [hashmap_main::hashmap::HashMap::{0}::allocate_slots]: decreases clause *)
 unfold
 let hashmap_hash_map_allocate_slots_decreases (t : Type0)
-  (slots : vec (hashmap_list_t t)) (n : usize) (st : state) : nat =
+  (slots : vec (hashmap_list_t t)) (n : usize) : nat =
   admit ()
 
 (** [hashmap_main::hashmap::HashMap::{0}::clear_slots]: decreases clause *)
 unfold
 let hashmap_hash_map_clear_slots_decreases (t : Type0)
-  (slots : vec (hashmap_list_t t)) (i : usize) (st : state) : nat =
+  (slots : vec (hashmap_list_t t)) (i : usize) : nat =
   admit ()
 
 (** [hashmap_main::hashmap::HashMap::{0}::insert_in_list]: decreases clause *)
 unfold
 let hashmap_hash_map_insert_in_list_decreases (t : Type0) (key : usize)
-  (value : t) (ls : hashmap_list_t t) (st : state) : nat =
+  (value : t) (ls : hashmap_list_t t) : nat =
   admit ()
 
 (** [hashmap_main::hashmap::HashMap::{0}::move_elements_from_list]: decreases clause *)
 unfold
 let hashmap_hash_map_move_elements_from_list_decreases (t : Type0)
-  (ntable : hashmap_hash_map_t t) (ls : hashmap_list_t t) (st : state) : nat =
+  (ntable : hashmap_hash_map_t t) (ls : hashmap_list_t t) : nat =
   admit ()
 
 (** [hashmap_main::hashmap::HashMap::{0}::move_elements]: decreases clause *)
 unfold
 let hashmap_hash_map_move_elements_decreases (t : Type0)
   (ntable : hashmap_hash_map_t t) (slots : vec (hashmap_list_t t)) (i : usize)
-  (st : state) : nat =
+  : nat =
   admit ()
 
 (** [hashmap_main::hashmap::HashMap::{0}::contains_key_in_list]: decreases clause *)
 unfold
 let hashmap_hash_map_contains_key_in_list_decreases (t : Type0) (key : usize)
-  (ls : hashmap_list_t t) (st : state) : nat =
+  (ls : hashmap_list_t t) : nat =
   admit ()
 
 (** [hashmap_main::hashmap::HashMap::{0}::get_in_list]: decreases clause *)
 unfold
 let hashmap_hash_map_get_in_list_decreases (t : Type0) (key : usize)
-  (ls : hashmap_list_t t) (st : state) : nat =
+  (ls : hashmap_list_t t) : nat =
   admit ()
 
 (** [hashmap_main::hashmap::HashMap::{0}::get_mut_in_list]: decreases clause *)
 unfold
 let hashmap_hash_map_get_mut_in_list_decreases (t : Type0) (key : usize)
-  (ls : hashmap_list_t t) (st : state) : nat =
+  (ls : hashmap_list_t t) : nat =
   admit ()
 
 (** [hashmap_main::hashmap::HashMap::{0}::remove_from_list]: decreases clause *)
 unfold
 let hashmap_hash_map_remove_from_list_decreases (t : Type0) (key : usize)
-  (ls : hashmap_list_t t) (st : state) : nat =
+  (ls : hashmap_list_t t) : nat =
   admit ()
 
