tests/hashmap_on_disk/HashmapMain.Funs.fst
@@ -9,17 +9,16 @@ include HashmapMain.Clauses
 #set-options "--z3rlimit 50 --fuel 0 --ifuel 1"
 
 (** [hashmap_main::hashmap::hash_key] *)
-let hashmap_hash_key_fwd (k : usize) (st : state) : result (state & usize) =
-  Return (st, k)
+let hashmap_hash_key_fwd (k : usize) : result usize = Return k
 
 (** [hashmap_main::hashmap::HashMap::{0}::allocate_slots] *)
 let rec hashmap_hash_map_allocate_slots_fwd
-  (t : Type0) (slots : vec (hashmap_list_t t)) (n : usize) (st : state) :
-  Tot (result (state & (vec (hashmap_list_t t))))
-  (decreases (hashmap_hash_map_allocate_slots_decreases t slots n st))
+  (t : Type0) (slots : vec (hashmap_list_t t)) (n : usize) :
+  Tot (result (vec (hashmap_list_t t)))
+  (decreases (hashmap_hash_map_allocate_slots_decreases t slots n))
   =
   begin match n with
-  | 0 -> Return (st, slots)
+  | 0 -> Return slots
   | _ ->
     begin match vec_push_back (hashmap_list_t t) slots HashmapListNil with
     | Fail -> Fail
@@ -27,9 +26,9 @@ let rec hashmap_hash_map_allocate_slots_fwd
       begin match usize_sub n 1 with
       | Fail -> Fail
       | Return i ->
-        begin match hashmap_hash_map_allocate_slots_fwd t slots0 i st with
+        begin match hashmap_hash_map_allocate_slots_fwd t slots0 i with
         | Fail -> Fail
-        | Return (st0, v) -> Return (st0, v)
+        | Return v -> Return v
         end
       end
     end
@@ -38,62 +37,37 @@ let rec hashmap_hash_map_allocate_slots_fwd
 (** [hashmap_main::hashmap::HashMap::{0}::new_with_capacity] *)
 let hashmap_hash_map_new_with_capacity_fwd
   (t : Type0) (capacity : usize) (max_load_dividend : usize)
-  (max_load_divisor : usize) (st : state) :
-  result (state & (hashmap_hash_map_t t))
+  (max_load_divisor : usize) :
+  result (hashmap_hash_map_t t)
   =
   let v = vec_new (hashmap_list_t t) in
-  begin match hashmap_hash_map_allocate_slots_fwd t v capacity st with
+  begin match hashmap_hash_map_allocate_slots_fwd t v capacity with
   | Fail -> Fail
-  | Return (st0, slots) ->
+  | Return slots ->
     begin match usize_mul capacity max_load_dividend with
     | Fail -> Fail
     | Return i ->
       begin match usize_div i max_load_divisor with
       | Fail -> Fail
       | Return i0 ->
-        Return (st0, Mkhashmap_hash_map_t 0 (max_load_dividend,
-          max_load_divisor) i0 slots)
+        Return (Mkhashmap_hash_map_t 0 (max_load_dividend, max_load_divisor) i0
+          slots)
       end
     end
   end
 
 (** [hashmap_main::hashmap::HashMap::{0}::new] *)
-let hashmap_hash_map_new_fwd
-  (t : Type0) (st : state) : result (state & (hashmap_hash_map_t t)) =
-  begin match hashmap_hash_map_new_with_capacity_fwd t 32 4 5 st with
+let hashmap_hash_map_new_fwd (t : Type0) : result (hashmap_hash_map_t t) =
+  begin match hashmap_hash_map_new_with_capacity_fwd t 32 4 5 with
   | Fail -> Fail
-  | Return (st0, hm) -> Return (st0, hm)
+  | Return hm -> Return hm
   end
 
 (** [hashmap_main::hashmap::HashMap::{0}::clear_slots] *)
-let rec hashmap_hash_map_clear_slots_fwd
-  (t : Type0) (slots : vec (hashmap_list_t t)) (i : usize) (st : state) :
-  Tot (result (state & unit))
-  (decreases (hashmap_hash_map_clear_slots_decreases t slots i st))
-  =
-  let i0 = vec_len (hashmap_list_t t) slots in
-  if i < i0
-  then
-    begin match vec_index_mut_back (hashmap_list_t t) slots i HashmapListNil
-      with
-    | Fail -> Fail
-    | Return slots0 ->
-      begin match usize_add i 1 with
-      | Fail -> Fail
-      | Return i1 ->
-        begin match hashmap_hash_map_clear_slots_fwd t slots0 i1 st with
-        | Fail -> Fail
-        | Return (st0, _) -> Return (st0, ())
-        end
-      end
-    end
-  else Return (st, ())
-
-(** [hashmap_main::hashmap::HashMap::{0}::clear_slots] *)
-let rec hashmap_hash_map_clear_slots_back
-  (t : Type0) (slots : vec (hashmap_list_t t)) (i : usize) (st : state) :
+let rec hashmap_hash_map_clear_slots_fwd_back
+  (t : Type0) (slots : vec (hashmap_list_t t)) (i : usize) :
   Tot (result (vec (hashmap_list_t t)))
-  (decreases (hashmap_hash_map_clear_slots_decreases t slots i st))
+  (decreases (hashmap_hash_map_clear_slots_decreases t slots i))
   =
   let i0 = vec_len (hashmap_list_t t) slots in
   if i < i0
@@ -105,7 +79,7 @@ let rec hashmap_hash_map_clear_slots_back
       begin match usize_add i 1 with
       | Fail -> Fail
       | Return i1 ->
-        begin match hashmap_hash_map_clear_slots_back t slots0 i1 st with
+        begin match hashmap_hash_map_clear_slots_fwd_back t slots0 i1 with
         | Fail -> Fail
         | Return slots1 -> Return slots1
         end
@@ -114,23 +88,10 @@ let rec hashmap_hash_map_clear_slots_back
   else Return slots
 
 (** [hashmap_main::hashmap::HashMap::{0}::clear] *)
-let hashmap_hash_map_clear_fwd
-  (t : Type0) (self : hashmap_hash_map_t t) (st : state) :
-  result (state & unit)
-  =
+let hashmap_hash_map_clear_fwd_back
+  (t : Type0) (self : hashmap_hash_map_t t) : result (hashmap_hash_map_t t) =
   begin match
-    hashmap_hash_map_clear_slots_fwd t self.hashmap_hash_map_slots 0 st with
-  | Fail -> Fail
-  | Return (st0, _) -> Return (st0, ())
-  end
-
-(** [hashmap_main::hashmap::HashMap::{0}::clear] *)
-let hashmap_hash_map_clear_back
-  (t : Type0) (self : hashmap_hash_map_t t) (st : state) :
-  result (hashmap_hash_map_t t)
-  =
-  begin match
-    hashmap_hash_map_clear_slots_back t self.hashmap_hash_map_slots 0 st with
+    hashmap_hash_map_clear_slots_fwd_back t self.hashmap_hash_map_slots 0 with
   | Fail -> Fail
   | Return v ->
     Return (Mkhashmap_hash_map_t 0 self.hashmap_hash_map_max_load_factor
@@ -139,41 +100,39 @@ let hashmap_hash_map_clear_back
 
 (** [hashmap_main::hashmap::HashMap::{0}::len] *)
 let hashmap_hash_map_len_fwd
-  (t : Type0) (self : hashmap_hash_map_t t) (st : state) :
-  result (state & usize)
-  =
-  Return (st, self.hashmap_hash_map_num_entries)
+  (t : Type0) (self : hashmap_hash_map_t t) : result usize =
+  Return self.hashmap_hash_map_num_entries
 
 (** [hashmap_main::hashmap::HashMap::{0}::insert_in_list] *)
 let rec hashmap_hash_map_insert_in_list_fwd
-  (t : Type0) (key : usize) (value : t) (ls : hashmap_list_t t) (st : state) :
-  Tot (result (state & bool))
-  (decreases (hashmap_hash_map_insert_in_list_decreases t key value ls st))
+  (t : Type0) (key : usize) (value : t) (ls : hashmap_list_t t) :
+  Tot (result bool)
+  (decreases (hashmap_hash_map_insert_in_list_decreases t key value ls))
   =
   begin match ls with
   | HashmapListCons ckey cvalue ls0 ->
     if ckey = key
-    then Return (st, false)
+    then Return false
     else
-      begin match hashmap_hash_map_insert_in_list_fwd t key value ls0 st with
+      begin match hashmap_hash_map_insert_in_list_fwd t key value ls0 with
       | Fail -> Fail
-      | Return (st0, b) -> Return (st0, b)
+      | Return b -> Return b
       end
-  | HashmapListNil -> Return (st, true)
+  | HashmapListNil -> Return true
   end
 
 (** [hashmap_main::hashmap::HashMap::{0}::insert_in_list] *)
 let rec hashmap_hash_map_insert_in_list_back
-  (t : Type0) (key : usize) (value : t) (ls : hashmap_list_t t) (st : state) :
+  (t : Type0) (key : usize) (value : t) (ls : hashmap_list_t t) :
   Tot (result (hashmap_list_t t))
-  (decreases (hashmap_hash_map_insert_in_list_decreases t key value ls st))
+  (decreases (hashmap_hash_map_insert_in_list_decreases t key value ls))
   =
   begin match ls with
   | HashmapListCons ckey cvalue ls0 ->
     if ckey = key
     then Return (HashmapListCons ckey value ls0)
     else
-      begin match hashmap_hash_map_insert_in_list_back t key value ls0 st with
+      begin match hashmap_hash_map_insert_in_list_back t key value ls0 with
       | Fail -> Fail
       | Return ls1 -> Return (HashmapListCons ckey cvalue ls1)
       end
@@ -182,47 +141,13 @@ let rec hashmap_hash_map_insert_in_list_back
   end
 
 (** [hashmap_main::hashmap::HashMap::{0}::insert_no_resize] *)
-let hashmap_hash_map_insert_no_resize_fwd
-  (t : Type0) (self : hashmap_hash_map_t t) (key : usize) (value : t)
-  (st : state) :
-  result (state & unit)
-  =
-  begin match hashmap_hash_key_fwd key st with
-  | Fail -> Fail
-  | Return (st0, hash) ->
-    let i = vec_len (hashmap_list_t t) self.hashmap_hash_map_slots in
-    begin match usize_rem hash i with
-    | Fail -> Fail
-    | Return hash_mod ->
-      begin match
-        vec_index_mut_fwd (hashmap_list_t t) self.hashmap_hash_map_slots
-          hash_mod with
-      | Fail -> Fail
-      | Return l ->
-        begin match hashmap_hash_map_insert_in_list_fwd t key value l st0 with
-        | Fail -> Fail
-        | Return (st1, inserted) ->
-          if inserted
-          then
-            begin match usize_add self.hashmap_hash_map_num_entries 1 with
-            | Fail -> Fail
-            | Return _ -> Return (st1, ())
-            end
-          else Return (st1, ())
-        end
-      end
-    end
-  end
-
-(** [hashmap_main::hashmap::HashMap::{0}::insert_no_resize] *)
-let hashmap_hash_map_insert_no_resize_back
-  (t : Type0) (self : hashmap_hash_map_t t) (key : usize) (value : t)
-  (st : state) :
+let hashmap_hash_map_insert_no_resize_fwd_back
+  (t : Type0) (self : hashmap_hash_map_t t) (key : usize) (value : t) :
   result (hashmap_hash_map_t t)
   =
-  begin match hashmap_hash_key_fwd key st with
+  begin match hashmap_hash_key_fwd key with
   | Fail -> Fail
-  | Return (st0, hash) ->
+  | Return hash ->
     let i = vec_len (hashmap_list_t t) self.hashmap_hash_map_slots in
     begin match usize_rem hash i with
     | Fail -> Fail
@@ -232,16 +157,16 @@ let hashmap_hash_map_insert_no_resize_back
           hash_mod with
       | Fail -> Fail
       | Return l ->
-        begin match hashmap_hash_map_insert_in_list_fwd t key value l st0 with
+        begin match hashmap_hash_map_insert_in_list_fwd t key value l with
         | Fail -> Fail
-        | Return (_, inserted) ->
+        | Return inserted ->
           if inserted
           then
             begin match usize_add self.hashmap_hash_map_num_entries 1 with
             | Fail -> Fail
             | Return i0 ->
-              begin match
-                hashmap_hash_map_insert_in_list_back t key value l st0 with
+              begin match hashmap_hash_map_insert_in_list_back t key value l
+                with
               | Fail -> Fail
               | Return l0 ->
                 begin match
@@ -256,8 +181,7 @@ let hashmap_hash_map_insert_no_resize_back
               end
             end
           else
-            begin match hashmap_hash_map_insert_in_list_back t key value l st0
-              with
+            begin match hashmap_hash_map_insert_in_list_back t key value l with
             | Fail -> Fail
             | Return l0 ->
               begin match
@@ -276,104 +200,31 @@ let hashmap_hash_map_insert_no_resize_back
   end
 
 (** [hashmap_main::hashmap::HashMap::{0}::move_elements_from_list] *)
-let rec hashmap_hash_map_move_elements_from_list_fwd
-  (t : Type0) (ntable : hashmap_hash_map_t t) (ls : hashmap_list_t t)
-  (st : state) :
-  Tot (result (state & unit))
-  (decreases (hashmap_hash_map_move_elements_from_list_decreases t ntable ls
-  st))
-  =
-  begin match ls with
-  | HashmapListCons k v tl ->
-    begin match hashmap_hash_map_insert_no_resize_fwd t ntable k v st with
-    | Fail -> Fail
-    | Return (st0, _) ->
-      begin match hashmap_hash_map_insert_no_resize_back t ntable k v st with
-      | Fail -> Fail
-      | Return ntable0 ->
-        begin match
-          hashmap_hash_map_move_elements_from_list_fwd t ntable0 tl st0 with
-        | Fail -> Fail
-        | Return (st1, _) -> Return (st1, ())
-        end
-      end
-    end
-  | HashmapListNil -> Return (st, ())
-  end
-
-(** [hashmap_main::hashmap::HashMap::{0}::move_elements_from_list] *)
-let rec hashmap_hash_map_move_elements_from_list_back
-  (t : Type0) (ntable : hashmap_hash_map_t t) (ls : hashmap_list_t t)
-  (st : state) :
+let rec hashmap_hash_map_move_elements_from_list_fwd_back
+  (t : Type0) (ntable : hashmap_hash_map_t t) (ls : hashmap_list_t t) :
   Tot (result (hashmap_hash_map_t t))
-  (decreases (hashmap_hash_map_move_elements_from_list_decreases t ntable ls
-  st))
+  (decreases (hashmap_hash_map_move_elements_from_list_decreases t ntable ls))
   =
   begin match ls with
   | HashmapListCons k v tl ->
-    begin match hashmap_hash_map_insert_no_resize_fwd t ntable k v st with
+    begin match hashmap_hash_map_insert_no_resize_fwd_back t ntable k v with
     | Fail -> Fail
-    | Return (st0, _) ->
-      begin match hashmap_hash_map_insert_no_resize_back t ntable k v st with
+    | Return ntable0 ->
+      begin match
+        hashmap_hash_map_move_elements_from_list_fwd_back t ntable0 tl with
       | Fail -> Fail
-      | Return ntable0 ->
-        begin match
-          hashmap_hash_map_move_elements_from_list_back t ntable0 tl st0 with
-        | Fail -> Fail
-        | Return ntable1 -> Return ntable1
-        end
+      | Return ntable1 -> Return ntable1
       end
     end
   | HashmapListNil -> Return ntable
   end
 
 (** [hashmap_main::hashmap::HashMap::{0}::move_elements] *)
-let rec hashmap_hash_map_move_elements_fwd
+let rec hashmap_hash_map_move_elements_fwd_back
   (t : Type0) (ntable : hashmap_hash_map_t t) (slots : vec (hashmap_list_t t))
-  (i : usize) (st : state) :
-  Tot (result (state & unit))
-  (decreases (hashmap_hash_map_move_elements_decreases t ntable slots i st))
-  =
-  let i0 = vec_len (hashmap_list_t t) slots in
-  if i < i0
-  then
-    begin match vec_index_mut_fwd (hashmap_list_t t) slots i with
-    | Fail -> Fail
-    | Return l ->
-      let ls = mem_replace_fwd (hashmap_list_t t) l HashmapListNil in
-      begin match hashmap_hash_map_move_elements_from_list_fwd t ntable ls st
-        with
-      | Fail -> Fail
-      | Return (st0, _) ->
-        begin match
-          hashmap_hash_map_move_elements_from_list_back t ntable ls st with
-        | Fail -> Fail
-        | Return ntable0 ->
-          let l0 = mem_replace_back (hashmap_list_t t) l HashmapListNil in
-          begin match vec_index_mut_back (hashmap_list_t t) slots i l0 with
-          | Fail -> Fail
-          | Return slots0 ->
-            begin match usize_add i 1 with
-            | Fail -> Fail
-            | Return i1 ->
-              begin match
-                hashmap_hash_map_move_elements_fwd t ntable0 slots0 i1 st0 with
-              | Fail -> Fail
-              | Return (st1, _) -> Return (st1, ())
-              end
-            end
-          end
-        end
-      end
-    end
-  else Return (st, ())
-
-(** [hashmap_main::hashmap::HashMap::{0}::move_elements] *)
-let rec hashmap_hash_map_move_elements_back
-  (t : Type0) (ntable : hashmap_hash_map_t t) (slots : vec (hashmap_list_t t))
-  (i : usize) (st : state) :
+  (i : usize) :
   Tot (result ((hashmap_hash_map_t t) & (vec (hashmap_list_t t))))
-  (decreases (hashmap_hash_map_move_elements_decreases t ntable slots i st))
+  (decreases (hashmap_hash_map_move_elements_decreases t ntable slots i))
   =
   let i0 = vec_len (hashmap_list_t t) slots in
   if i < i0
@@ -382,27 +233,21 @@ let rec hashmap_hash_map_move_elements_back
     | Fail -> Fail
     | Return l ->
       let ls = mem_replace_fwd (hashmap_list_t t) l HashmapListNil in
-      begin match hashmap_hash_map_move_elements_from_list_fwd t ntable ls st
+      begin match hashmap_hash_map_move_elements_from_list_fwd_back t ntable ls
         with
       | Fail -> Fail
-      | Return (st0, _) ->
-        begin match
-          hashmap_hash_map_move_elements_from_list_back t ntable ls st with
+      | Return ntable0 ->
+        let l0 = mem_replace_back (hashmap_list_t t) l HashmapListNil in
+        begin match vec_index_mut_back (hashmap_list_t t) slots i l0 with
         | Fail -> Fail
-        | Return ntable0 ->
-          let l0 = mem_replace_back (hashmap_list_t t) l HashmapListNil in
-          begin match vec_index_mut_back (hashmap_list_t t) slots i l0 with
+        | Return slots0 ->
+          begin match usize_add i 1 with
           | Fail -> Fail
-          | Return slots0 ->
-            begin match usize_add i 1 with
+          | Return i1 ->
+            begin match
+              hashmap_hash_map_move_elements_fwd_back t ntable0 slots0 i1 with
             | Fail -> Fail
-            | Return i1 ->
-              begin match
-                hashmap_hash_map_move_elements_back t ntable0 slots0 i1 st0
-                with
-              | Fail -> Fail
-              | Return (ntable1, slots1) -> Return (ntable1, slots1)
-              end
+            | Return (ntable1, slots1) -> Return (ntable1, slots1)
             end
           end
         end
@@ -411,10 +256,8 @@ let rec hashmap_hash_map_move_elements_back
   else Return (ntable, slots)
 
 (** [hashmap_main::hashmap::HashMap::{0}::try_resize] *)
-let hashmap_hash_map_try_resize_fwd
-  (t : Type0) (self : hashmap_hash_map_t t) (st : state) :
-  result (state & unit)
-  =
+let hashmap_hash_map_try_resize_fwd_back
+  (t : Type0) (self : hashmap_hash_map_t t) : result (hashmap_hash_map_t t) =
   let capacity = vec_len (hashmap_list_t t) self.hashmap_hash_map_slots in
   begin match usize_div 4294967295 2 with
   | Fail -> Fail
@@ -428,51 +271,12 @@ let hashmap_hash_map_try_resize_fwd
         begin match usize_mul capacity 2 with
         | Fail -> Fail
         | Return i2 ->
-          begin match hashmap_hash_map_new_with_capacity_fwd t i2 i i0 st with
+          begin match hashmap_hash_map_new_with_capacity_fwd t i2 i i0 with
           | Fail -> Fail
-          | Return (st0, ntable) ->
+          | Return ntable ->
             begin match
-              hashmap_hash_map_move_elements_fwd t ntable
-                self.hashmap_hash_map_slots 0 st0 with
-            | Fail -> Fail
-            | Return (st1, _) ->
-              begin match
-                hashmap_hash_map_move_elements_back t ntable
-                  self.hashmap_hash_map_slots 0 st0 with
-              | Fail -> Fail
-              | Return (_, _) -> Return (st1, ())
-              end
-            end
-          end
-        end
-      else Return (st, ())
-    end
-  end
-
-(** [hashmap_main::hashmap::HashMap::{0}::try_resize] *)
-let hashmap_hash_map_try_resize_back
-  (t : Type0) (self : hashmap_hash_map_t t) (st : state) :
-  result (hashmap_hash_map_t t)
-  =
-  let capacity = vec_len (hashmap_list_t t) self.hashmap_hash_map_slots in
-  begin match usize_div 4294967295 2 with
-  | Fail -> Fail
-  | Return n1 ->
-    let (i, i0) = self.hashmap_hash_map_max_load_factor in
-    begin match usize_div n1 i with
-    | Fail -> Fail
-    | Return i1 ->
-      if capacity <= i1
-      then
-        begin match usize_mul capacity 2 with
-        | Fail -> Fail
-        | Return i2 ->
-          begin match hashmap_hash_map_new_with_capacity_fwd t i2 i i0 st with
-          | Fail -> Fail
-          | Return (st0, ntable) ->
-            begin match
-              hashmap_hash_map_move_elements_back t ntable
-                self.hashmap_hash_map_slots 0 st0 with
+              hashmap_hash_map_move_elements_fwd_back t ntable
+                self.hashmap_hash_map_slots 0 with
             | Fail -> Fail
             | Return (ntable0, _) ->
               Return (Mkhashmap_hash_map_t self.hashmap_hash_map_num_entries
@@ -488,96 +292,57 @@ let hashmap_hash_map_try_resize_back
   end
 
 (** [hashmap_main::hashmap::HashMap::{0}::insert] *)
-let hashmap_hash_map_insert_fwd
-  (t : Type0) (self : hashmap_hash_map_t t) (key : usize) (value : t)
-  (st : state) :
-  result (state & unit)
-  =
-  begin match hashmap_hash_map_insert_no_resize_fwd t self key value st with
-  | Fail -> Fail
-  | Return (st0, _) ->
-    begin match hashmap_hash_map_insert_no_resize_back t self key value st with
-    | Fail -> Fail
-    | Return self0 ->
-      begin match hashmap_hash_map_len_fwd t self0 st0 with
-      | Fail -> Fail
-      | Return (st1, i) ->
-        if i > self0.hashmap_hash_map_max_load
-        then
-          begin match
-            hashmap_hash_map_try_resize_fwd t (Mkhashmap_hash_map_t
-              self0.hashmap_hash_map_num_entries
-              self0.hashmap_hash_map_max_load_factor
-              self0.hashmap_hash_map_max_load self0.hashmap_hash_map_slots) st1
-            with
-          | Fail -> Fail
-          | Return (st2, _) -> Return (st2, ())
-          end
-        else Return (st1, ())
-      end
-    end
-  end
-
-(** [hashmap_main::hashmap::HashMap::{0}::insert] *)
-let hashmap_hash_map_insert_back
-  (t : Type0) (self : hashmap_hash_map_t t) (key : usize) (value : t)
-  (st : state) :
+let hashmap_hash_map_insert_fwd_back
+  (t : Type0) (self : hashmap_hash_map_t t) (key : usize) (value : t) :
   result (hashmap_hash_map_t t)
   =
-  begin match hashmap_hash_map_insert_no_resize_fwd t self key value st with
+  begin match hashmap_hash_map_insert_no_resize_fwd_back t self key value with
   | Fail -> Fail
-  | Return (st0, _) ->
-    begin match hashmap_hash_map_insert_no_resize_back t self key value st with
+  | Return self0 ->
+    begin match hashmap_hash_map_len_fwd t self0 with
     | Fail -> Fail
-    | Return self0 ->
-      begin match hashmap_hash_map_len_fwd t self0 st0 with
-      | Fail -> Fail
-      | Return (st1, i) ->
-        if i > self0.hashmap_hash_map_max_load
-        then
-          begin match
-            hashmap_hash_map_try_resize_back t (Mkhashmap_hash_map_t
-              self0.hashmap_hash_map_num_entries
-              self0.hashmap_hash_map_max_load_factor
-              self0.hashmap_hash_map_max_load self0.hashmap_hash_map_slots) st1
-            with
-          | Fail -> Fail
-          | Return self1 -> Return self1
-          end
-        else
-          Return (Mkhashmap_hash_map_t self0.hashmap_hash_map_num_entries
+    | Return i ->
+      if i > self0.hashmap_hash_map_max_load
+      then
+        begin match
+          hashmap_hash_map_try_resize_fwd_back t (Mkhashmap_hash_map_t
+            self0.hashmap_hash_map_num_entries
             self0.hashmap_hash_map_max_load_factor
-            self0.hashmap_hash_map_max_load self0.hashmap_hash_map_slots)
-      end
+            self0.hashmap_hash_map_max_load self0.hashmap_hash_map_slots) with
+        | Fail -> Fail
+        | Return self1 -> Return self1
+        end
+      else
+        Return (Mkhashmap_hash_map_t self0.hashmap_hash_map_num_entries
+          self0.hashmap_hash_map_max_load_factor
+          self0.hashmap_hash_map_max_load self0.hashmap_hash_map_slots)
     end
   end
 
 (** [hashmap_main::hashmap::HashMap::{0}::contains_key_in_list] *)
 let rec hashmap_hash_map_contains_key_in_list_fwd
-  (t : Type0) (key : usize) (ls : hashmap_list_t t) (st : state) :
-  Tot (result (state & bool))
-  (decreases (hashmap_hash_map_contains_key_in_list_decreases t key ls st))
+  (t : Type0) (key : usize) (ls : hashmap_list_t t) :
+  Tot (result bool)
+  (decreases (hashmap_hash_map_contains_key_in_list_decreases t key ls))
   =
   begin match ls with
   | HashmapListCons ckey x ls0 ->
     if ckey = key
-    then Return (st, true)
+    then Return true
     else
-      begin match hashmap_hash_map_contains_key_in_list_fwd t key ls0 st with
+      begin match hashmap_hash_map_contains_key_in_list_fwd t key ls0 with
       | Fail -> Fail
-      | Return (st0, b) -> Return (st0, b)
+      | Return b -> Return b
       end
-  | HashmapListNil -> Return (st, false)
+  | HashmapListNil -> Return false
   end
 
 (** [hashmap_main::hashmap::HashMap::{0}::contains_key] *)
 let hashmap_hash_map_contains_key_fwd
-  (t : Type0) (self : hashmap_hash_map_t t) (key : usize) (st : state) :
-  result (state & bool)
-  =
-  begin match hashmap_hash_key_fwd key st with
+  (t : Type0) (self : hashmap_hash_map_t t) (key : usize) : result bool =
+  begin match hashmap_hash_key_fwd key with
   | Fail -> Fail
-  | Return (st0, hash) ->
+  | Return hash ->
     let i = vec_len (hashmap_list_t t) self.hashmap_hash_map_slots in
     begin match usize_rem hash i with
     | Fail -> Fail
@@ -587,9 +352,9 @@ let hashmap_hash_map_contains_key_fwd
         with
       | Fail -> Fail
       | Return l ->
-        begin match hashmap_hash_map_contains_key_in_list_fwd t key l st0 with
+        begin match hashmap_hash_map_contains_key_in_list_fwd t key l with
         | Fail -> Fail
-        | Return (st1, b) -> Return (st1, b)
+        | Return b -> Return b
         end
       end
     end
@@ -597,30 +362,27 @@ let hashmap_hash_map_contains_key_fwd
 
 (** [hashmap_main::hashmap::HashMap::{0}::get_in_list] *)
 let rec hashmap_hash_map_get_in_list_fwd
-  (t : Type0) (key : usize) (ls : hashmap_list_t t) (st : state) :
-  Tot (result (state & t))
-  (decreases (hashmap_hash_map_get_in_list_decreases t key ls st))
+  (t : Type0) (key : usize) (ls : hashmap_list_t t) :
+  Tot (result t) (decreases (hashmap_hash_map_get_in_list_decreases t key ls))
   =
   begin match ls with
   | HashmapListCons ckey cvalue ls0 ->
     if ckey = key
-    then Return (st, cvalue)
+    then Return cvalue
     else
-      begin match hashmap_hash_map_get_in_list_fwd t key ls0 st with
+      begin match hashmap_hash_map_get_in_list_fwd t key ls0 with
       | Fail -> Fail
-      | Return (st0, x) -> Return (st0, x)
+      | Return x -> Return x
       end
   | HashmapListNil -> Fail
   end
 
 (** [hashmap_main::hashmap::HashMap::{0}::get] *)
 let hashmap_hash_map_get_fwd
-  (t : Type0) (self : hashmap_hash_map_t t) (key : usize) (st : state) :
-  result (state & t)
-  =
-  begin match hashmap_hash_key_fwd key st with
+  (t : Type0) (self : hashmap_hash_map_t t) (key : usize) : result t =
+  begin match hashmap_hash_key_fwd key with
   | Fail -> Fail
-  | Return (st0, hash) ->
+  | Return hash ->
     let i = vec_len (hashmap_list_t t) self.hashmap_hash_map_slots in
     begin match usize_rem hash i with
     | Fail -> Fail
@@ -630,9 +392,9 @@ let hashmap_hash_map_get_fwd
         with
       | Fail -> Fail
       | Return l ->
-        begin match hashmap_hash_map_get_in_list_fwd t key l st0 with
+        begin match hashmap_hash_map_get_in_list_fwd t key l with
         | Fail -> Fail
-        | Return (st1, x) -> Return (st1, x)
+        | Return x -> Return x
         end
       end
     end
@@ -640,34 +402,34 @@ let hashmap_hash_map_get_fwd
 
 (** [hashmap_main::hashmap::HashMap::{0}::get_mut_in_list] *)
 let rec hashmap_hash_map_get_mut_in_list_fwd
-  (t : Type0) (key : usize) (ls : hashmap_list_t t) (st : state) :
-  Tot (result (state & t))
-  (decreases (hashmap_hash_map_get_mut_in_list_decreases t key ls st))
+  (t : Type0) (key : usize) (ls : hashmap_list_t t) :
+  Tot (result t)
+  (decreases (hashmap_hash_map_get_mut_in_list_decreases t key ls))
   =
   begin match ls with
   | HashmapListCons ckey cvalue ls0 ->
     if ckey = key
-    then Return (st, cvalue)
+    then Return cvalue
     else
-      begin match hashmap_hash_map_get_mut_in_list_fwd t key ls0 st with
+      begin match hashmap_hash_map_get_mut_in_list_fwd t key ls0 with
       | Fail -> Fail
-      | Return (st0, x) -> Return (st0, x)
+      | Return x -> Return x
       end
   | HashmapListNil -> Fail
   end
 
 (** [hashmap_main::hashmap::HashMap::{0}::get_mut_in_list] *)
 let rec hashmap_hash_map_get_mut_in_list_back
-  (t : Type0) (key : usize) (ls : hashmap_list_t t) (st : state) (ret : t) :
+  (t : Type0) (key : usize) (ls : hashmap_list_t t) (ret : t) :
   Tot (result (hashmap_list_t t))
-  (decreases (hashmap_hash_map_get_mut_in_list_decreases t key ls st))
+  (decreases (hashmap_hash_map_get_mut_in_list_decreases t key ls))
   =
   begin match ls with
   | HashmapListCons ckey cvalue ls0 ->
     if ckey = key
     then Return (HashmapListCons ckey ret ls0)
     else
-      begin match hashmap_hash_map_get_mut_in_list_back t key ls0 st ret with
+      begin match hashmap_hash_map_get_mut_in_list_back t key ls0 ret with
       | Fail -> Fail
       | Return ls1 -> Return (HashmapListCons ckey cvalue ls1)
       end
@@ -676,12 +438,10 @@ let rec hashmap_hash_map_get_mut_in_list_back
 
 (** [hashmap_main::hashmap::HashMap::{0}::get_mut] *)
 let hashmap_hash_map_get_mut_fwd
-  (t : Type0) (self : hashmap_hash_map_t t) (key : usize) (st : state) :
-  result (state & t)
-  =
-  begin match hashmap_hash_key_fwd key st with
+  (t : Type0) (self : hashmap_hash_map_t t) (key : usize) : result t =
+  begin match hashmap_hash_key_fwd key with
   | Fail -> Fail
-  | Return (st0, hash) ->
+  | Return hash ->
     let i = vec_len (hashmap_list_t t) self.hashmap_hash_map_slots in
     begin match usize_rem hash i with
     | Fail -> Fail
@@ -691,9 +451,9 @@ let hashmap_hash_map_get_mut_fwd
           hash_mod with
       | Fail -> Fail
       | Return l ->
-        begin match hashmap_hash_map_get_mut_in_list_fwd t key l st0 with
+        begin match hashmap_hash_map_get_mut_in_list_fwd t key l with
         | Fail -> Fail
-        | Return (st1, x) -> Return (st1, x)
+        | Return x -> Return x
         end
       end
     end
@@ -701,13 +461,12 @@ let hashmap_hash_map_get_mut_fwd
 
 (** [hashmap_main::hashmap::HashMap::{0}::get_mut] *)
 let hashmap_hash_map_get_mut_back
-  (t : Type0) (self : hashmap_hash_map_t t) (key : usize) (st : state)
-  (ret : t) :
+  (t : Type0) (self : hashmap_hash_map_t t) (key : usize) (ret : t) :
   result (hashmap_hash_map_t t)
   =
-  begin match hashmap_hash_key_fwd key st with
+  begin match hashmap_hash_key_fwd key with
   | Fail -> Fail
-  | Return (st0, hash) ->
+  | Return hash ->
     let i = vec_len (hashmap_list_t t) self.hashmap_hash_map_slots in
     begin match usize_rem hash i with
     | Fail -> Fail
@@ -717,7 +476,7 @@ let hashmap_hash_map_get_mut_back
           hash_mod with
       | Fail -> Fail
       | Return l ->
-        begin match hashmap_hash_map_get_mut_in_list_back t key l st0 ret with
+        begin match hashmap_hash_map_get_mut_in_list_back t key l ret with
         | Fail -> Fail
         | Return l0 ->
           begin match
@@ -736,9 +495,9 @@ let hashmap_hash_map_get_mut_back
 
 (** [hashmap_main::hashmap::HashMap::{0}::remove_from_list] *)
 let rec hashmap_hash_map_remove_from_list_fwd
-  (t : Type0) (key : usize) (ls : hashmap_list_t t) (st : state) :
-  Tot (result (state & (option t)))
-  (decreases (hashmap_hash_map_remove_from_list_decreases t key ls st))
+  (t : Type0) (key : usize) (ls : hashmap_list_t t) :
+  Tot (result (option t))
+  (decreases (hashmap_hash_map_remove_from_list_decreases t key ls))
   =
   begin match ls with
   | HashmapListCons ckey x tl ->
@@ -748,22 +507,22 @@ let rec hashmap_hash_map_remove_from_list_fwd
         mem_replace_fwd (hashmap_list_t t) (HashmapListCons ckey x tl)
           HashmapListNil in
       begin match mv_ls with
-      | HashmapListCons i cvalue tl0 -> Return (st, Some cvalue)
+      | HashmapListCons i cvalue tl0 -> Return (Some cvalue)
       | HashmapListNil -> Fail
       end
     else
-      begin match hashmap_hash_map_remove_from_list_fwd t key tl st with
+      begin match hashmap_hash_map_remove_from_list_fwd t key tl with
       | Fail -> Fail
-      | Return (st0, opt) -> Return (st0, opt)
+      | Return opt -> Return opt
       end
-  | HashmapListNil -> Return (st, None)
+  | HashmapListNil -> Return None
   end
 
 (** [hashmap_main::hashmap::HashMap::{0}::remove_from_list] *)
 let rec hashmap_hash_map_remove_from_list_back
-  (t : Type0) (key : usize) (ls : hashmap_list_t t) (st : state) :
+  (t : Type0) (key : usize) (ls : hashmap_list_t t) :
   Tot (result (hashmap_list_t t))
-  (decreases (hashmap_hash_map_remove_from_list_decreases t key ls st))
+  (decreases (hashmap_hash_map_remove_from_list_decreases t key ls))
   =
   begin match ls with
   | HashmapListCons ckey x tl ->
@@ -777,7 +536,7 @@ let rec hashmap_hash_map_remove_from_list_back
       | HashmapListNil -> Fail
       end
     else
-      begin match hashmap_hash_map_remove_from_list_back t key tl st with
+      begin match hashmap_hash_map_remove_from_list_back t key tl with
       | Fail -> Fail
       | Return tl0 -> Return (HashmapListCons ckey x tl0)
       end
@@ -786,12 +545,10 @@ let rec hashmap_hash_map_remove_from_list_back
 
 (** [hashmap_main::hashmap::HashMap::{0}::remove] *)
 let hashmap_hash_map_remove_fwd
-  (t : Type0) (self : hashmap_hash_map_t t) (key : usize) (st : state) :
-  result (state & (option t))
-  =
-  begin match hashmap_hash_key_fwd key st with
+  (t : Type0) (self : hashmap_hash_map_t t) (key : usize) : result (option t) =
+  begin match hashmap_hash_key_fwd key with
   | Fail -> Fail
-  | Return (st0, hash) ->
+  | Return hash ->
     let i = vec_len (hashmap_list_t t) self.hashmap_hash_map_slots in
     begin match usize_rem hash i with
     | Fail -> Fail
@@ -801,15 +558,15 @@ let hashmap_hash_map_remove_fwd
           hash_mod with
       | Fail -> Fail
       | Return l ->
-        begin match hashmap_hash_map_remove_from_list_fwd t key l st0 with
+        begin match hashmap_hash_map_remove_from_list_fwd t key l with
         | Fail -> Fail
-        | Return (st1, x) ->
+        | Return x ->
           begin match x with
-          | None -> Return (st1, None)
+          | None -> Return None
           | Some x0 ->
             begin match usize_sub self.hashmap_hash_map_num_entries 1 with
             | Fail -> Fail
-            | Return _ -> Return (st1, Some x0)
+            | Return _ -> Return (Some x0)
             end
           end
         end
@@ -819,12 +576,12 @@ let hashmap_hash_map_remove_fwd
 
 (** [hashmap_main::hashmap::HashMap::{0}::remove] *)
 let hashmap_hash_map_remove_back
-  (t : Type0) (self : hashmap_hash_map_t t) (key : usize) (st : state) :
+  (t : Type0) (self : hashmap_hash_map_t t) (key : usize) :
   result (hashmap_hash_map_t t)
   =
-  begin match hashmap_hash_key_fwd key st with
+  begin match hashmap_hash_key_fwd key with
   | Fail -> Fail
-  | Return (st0, hash) ->
+  | Return hash ->
     let i = vec_len (hashmap_list_t t) self.hashmap_hash_map_slots in
     begin match usize_rem hash i with
     | Fail -> Fail
@@ -834,12 +591,12 @@ let hashmap_hash_map_remove_back
           hash_mod with
       | Fail -> Fail
       | Return l ->
-        begin match hashmap_hash_map_remove_from_list_fwd t key l st0 with
+        begin match hashmap_hash_map_remove_from_list_fwd t key l with
         | Fail -> Fail
-        | Return (_, x) ->
+        | Return x ->
           begin match x with
           | None ->
-            begin match hashmap_hash_map_remove_from_list_back t key l st0 with
+            begin match hashmap_hash_map_remove_from_list_back t key l with
             | Fail -> Fail
             | Return l0 ->
               begin match
@@ -856,8 +613,7 @@ let hashmap_hash_map_remove_back
             begin match usize_sub self.hashmap_hash_map_num_entries 1 with
             | Fail -> Fail
             | Return i0 ->
-              begin match hashmap_hash_map_remove_from_list_back t key l st0
-                with
+              begin match hashmap_hash_map_remove_from_list_back t key l with
               | Fail -> Fail
               | Return l0 ->
                 begin match
@@ -878,112 +634,80 @@ let hashmap_hash_map_remove_back
   end
 
 (** [hashmap_main::hashmap::test1] *)
-let hashmap_test1_fwd (st : state) : result (state & unit) =
-  begin match hashmap_hash_map_new_fwd u64 st with
+let hashmap_test1_fwd : result unit =
+  begin match hashmap_hash_map_new_fwd u64 with
   | Fail -> Fail
-  | Return (st0, hm) ->
-    begin match hashmap_hash_map_insert_fwd u64 hm 0 42 st0 with
+  | Return hm ->
+    begin match hashmap_hash_map_insert_fwd_back u64 hm 0 42 with
     | Fail -> Fail
-    | Return (st1, _) ->
-      begin match hashmap_hash_map_insert_back u64 hm 0 42 st0 with
+    | Return hm0 ->
+      begin match hashmap_hash_map_insert_fwd_back u64 hm0 128 18 with
       | Fail -> Fail
-      | Return hm0 ->
-        begin match hashmap_hash_map_insert_fwd u64 hm0 128 18 st1 with
+      | Return hm1 ->
+        begin match hashmap_hash_map_insert_fwd_back u64 hm1 1024 138 with
         | Fail -> Fail
-        | Return (st2, _) ->
-          begin match hashmap_hash_map_insert_back u64 hm0 128 18 st1 with
+        | Return hm2 ->
+          begin match hashmap_hash_map_insert_fwd_back u64 hm2 1056 256 with
           | Fail -> Fail
-          | Return hm1 ->
-            begin match hashmap_hash_map_insert_fwd u64 hm1 1024 138 st2 with
+          | Return hm3 ->
+            begin match hashmap_hash_map_get_fwd u64 hm3 128 with
             | Fail -> Fail
-            | Return (st3, _) ->
-              begin match hashmap_hash_map_insert_back u64 hm1 1024 138 st2
-                with
-              | Fail -> Fail
-              | Return hm2 ->
-                begin match hashmap_hash_map_insert_fwd u64 hm2 1056 256 st3
-                  with
+            | Return i ->
+              if not (i = 18)
+              then Fail
+              else
+                begin match hashmap_hash_map_get_mut_back u64 hm3 1024 56 with
                 | Fail -> Fail
-                | Return (st4, _) ->
-                  begin match hashmap_hash_map_insert_back u64 hm2 1056 256 st3
-                    with
+                | Return hm4 ->
+                  begin match hashmap_hash_map_get_fwd u64 hm4 1024 with
                   | Fail -> Fail
-                  | Return hm3 ->
-                    begin match hashmap_hash_map_get_fwd u64 hm3 128 st4 with
-                    | Fail -> Fail
-                    | Return (st5, i) ->
-                      if not (i = 18)
-                      then Fail
-                      else
-                        begin match
-                          hashmap_hash_map_get_mut_fwd u64 hm3 1024 st5 with
-                        | Fail -> Fail
-                        | Return (st6, _) ->
-                          begin match
-                            hashmap_hash_map_get_mut_back u64 hm3 1024 st5 56
-                            with
-                          | Fail -> Fail
-                          | Return hm4 ->
+                  | Return i0 ->
+                    if not (i0 = 56)
+                    then Fail
+                    else
+                      begin match hashmap_hash_map_remove_fwd u64 hm4 1024 with
+                      | Fail -> Fail
+                      | Return x ->
+                        begin match x with
+                        | None -> Fail
+                        | Some x0 ->
+                          if not (x0 = 56)
+                          then Fail
+                          else
                             begin match
-                              hashmap_hash_map_get_fwd u64 hm4 1024 st6 with
+                              hashmap_hash_map_remove_back u64 hm4 1024 with
                             | Fail -> Fail
-                            | Return (st7, i0) ->
-                              if not (i0 = 56)
-                              then Fail
-                              else
-                                begin match
-                                  hashmap_hash_map_remove_fwd u64 hm4 1024 st7
-                                  with
-                                | Fail -> Fail
-                                | Return (st8, x) ->
-                                  begin match x with
-                                  | None -> Fail
-                                  | Some x0 ->
-                                    if not (x0 = 56)
+                            | Return hm5 ->
+                              begin match hashmap_hash_map_get_fwd u64 hm5 0
+                                with
+                              | Fail -> Fail
+                              | Return i1 ->
+                                if not (i1 = 42)
+                                then Fail
+                                else
+                                  begin match
+                                    hashmap_hash_map_get_fwd u64 hm5 128 with
+                                  | Fail -> Fail
+                                  | Return i2 ->
+                                    if not (i2 = 18)
                                     then Fail
                                     else
                                       begin match
-                                        hashmap_hash_map_remove_back u64 hm4
-                                          1024 st7 with
+                                        hashmap_hash_map_get_fwd u64 hm5 1056
+                                        with
                                       | Fail -> Fail
-                                      | Return hm5 ->
-                                        begin match
-                                          hashmap_hash_map_get_fwd u64 hm5 0
-                                            st8 with
-                                        | Fail -> Fail
-                                        | Return (st9, i1) ->
-                                          if not (i1 = 42)
-                                          then Fail
-                                          else
-                                            begin match
-                                              hashmap_hash_map_get_fwd u64 hm5
-                                                128 st9 with
-                                            | Fail -> Fail
-                                            | Return (st10, i2) ->
-                                              if not (i2 = 18)
-                                              then Fail
-                                              else
-                                                begin match
-                                                  hashmap_hash_map_get_fwd u64
-                                                    hm5 1056 st10 with
-                                                | Fail -> Fail
-                                                | Return (st11, i3) ->
-                                                  if not (i3 = 256)
-                                                  then Fail
-                                                  else Return (st11, ())
-                                                end
-                                            end
-                                        end
+                                      | Return i3 ->
+                                        if not (i3 = 256)
+                                        then Fail
+                                        else Return ()
                                       end
                                   end
-                                end
+                              end
                             end
-                          end
                         end
-                    end
+                      end
                   end
                 end
-              end
             end
           end
         end
@@ -991,26 +715,28 @@ let hashmap_test1_fwd (st : state) : result (state & unit) =
     end
   end
 
+(** Unit test for [hashmap_main::hashmap::test1] *)
+let _ = assert_norm (hashmap_test1_fwd = Return ())
+
 (** [hashmap_main::insert_on_disk] *)
 let insert_on_disk_fwd
   (key : usize) (value : u64) (st : state) : result (state & unit) =
   begin match hashmap_utils_deserialize_fwd st with
   | Fail -> Fail
   | Return (st0, hm) ->
-    begin match hashmap_hash_map_insert_fwd u64 hm key value st0 with
+    begin match hashmap_hash_map_insert_fwd_back u64 hm key value with
     | Fail -> Fail
-    | Return (st1, _) ->
-      begin match hashmap_hash_map_insert_back u64 hm key value st0 with
+    | Return hm0 ->
+      begin match hashmap_utils_serialize_fwd hm0 st0 with
       | Fail -> Fail
-      | Return hm0 ->
-        begin match hashmap_utils_serialize_fwd hm0 st1 with
-        | Fail -> Fail
-        | Return (st2, _) -> Return (st2, ())
-        end
+      | Return (st1, _) -> Return (st1, ())
       end
     end
   end
 
 (** [hashmap_main::main] *)
-let main_fwd (st : state) : result (state & unit) = Return (st, ())
+let main_fwd : result unit = Return ()
+
+(** Unit test for [hashmap_main::main] *)
+let _ = assert_norm (main_fwd = Return ())
 
